Cheat to get unification on arguments for free

theories/Irr/Irr.v
@@ -1,16 +1,23 @@
+(** I cheat, unification is not able to do anything with the primitives
+     but by using constants as synonym, it works :-) *)
+Definition Irr := Irr_prim.
+Definition iPrf (P: Irr) := iPrf_prim P.
+Definition iJMeq {A B} (a : A) (b : B) := iJMeq_prim a b.
+Definition isubst {A} (a b: A) (eq: iPrf (iJMeq a b)) (P: A -> Type)
+  (p: P a) := isubst_prim a b eq P p.
+
 Definition ireflTY A (a : A) : Irr := iJMeq a a.
 
-Axiom irefl : forall A a, iPrf (ireflTY A a).
+Axiom irefl : forall {A} a, iPrf (ireflTY A a).
 Axiom iAll : forall (S : Type) (P : S -> Irr), Irr.
-
-Definition casK A a (p : iPrf (ireflTY A a)): p = irefl A a :=
+Definition casK A a (p : iPrf (ireflTY A a)): p = irefl a :=
   eq_refl.
 
 Fixpoint iplus_n_Sm (m n : nat) : iPrf (iJMeq (m + S n) (S m + n)) :=
-match m return iPrf (iJMeq (m + S n) (S m + n)) with
-  | 0 => irefl _ (S n)
-  | S m' => isubst (m' + S n) (S m' + n) (iplus_n_Sm m' n) (fun x : nat => iPrf (iJMeq (S m' + S n) (S x)))
-    (irefl _ (S m' + S n))
+match m with
+  | 0 => irefl (S n)
+  | S m' => isubst _ _ (iplus_n_Sm m' n) (fun x : nat => iPrf (iJMeq (S m' + S n) (S x)))
+    (irefl (S m' + S n))
 end.
 
 Require Plus.
@@ -18,10 +25,10 @@ Require Plus.
 Lemma iplus_tail_plus m : forall n, iPrf (iJMeq (Plus.tail_plus m n) (m + n)).
 Proof.
 induction m.
-exact (fun n => irefl _ n).
+exact irefl.
 intro n.
-refine ((fun a => isubst (m + S n) (S m + n) (iplus_n_Sm m n)
-  (fun x : nat => iPrf (iJMeq (Plus.tail_plus (S m) n) x)) a) _).
+refine (isubst _ _ (iplus_n_Sm m n)
+  (fun x : nat => iPrf (iJMeq (Plus.tail_plus (S m) n) x)) _).
 exact (IHm (S n)).
 Qed.
 
@@ -43,7 +50,6 @@ Eval lazy in (Vector.rev_append (0 :: v'1) v'2).
 Eval lazy in (irev_append (0 :: v1) v2).
 Eval lazy in (irev_append (0 :: v'1) v'2).
 
-Definition useless m n (f : Fin.t (S (n + m))) :=
-  isubst (S (n + m)) (S n + m) (irefl nat (S (n + m))) Fin.t f.
+Definition useless m n (f : Fin.t (S (n + m))) := isubst _ _ (irefl (S (n + m))) Fin.t f.
 
 End test_suite.
